Typing Algorithm correctness

Rocq/src/Equiv.v
@@ -2,7 +2,7 @@ From Stdlib Require Import Lists.List.
 From Stdlib Require Import PeanoNat.
 
 From Verilog Require Import Expr.
-From Verilog Require Import Path.
+From Verilog Require Import ExprPath.
 From Verilog Require Import Spec.
 From Verilog Require Import TypeSystem.
 From Verilog Require Import Utils.
@@ -11,248 +11,107 @@ Import ListNotations.
 Import Nat.
 
 Import Expr.
+Import ExprPath.
 Import Path.
 Import Spec.
 Import TypeSystem.
 Import Utils.
 
-Set Implicit Arguments.
-
 Module Equiv.
 
-  Theorem spec_implies_ts : forall f1,
-      propagate_def f1 -> forall e f2, e ==> (determine e) -| f2 ->
-                                 forall p, IsPath e p -> forall n, f1 e p = n -> f2 p = Some n.
+  Definition agree e f1 (f2: path -> option nat) :=
+    forall p, IsPath e p -> f2 p = Some (f1 p).
+
+  Ltac antisym :=
+    match goal with
+    | [ H: ?x <= ?y, F: ?y <= ?x |- _ ] =>
+        let nH := fresh in assert (nH: x = y) by apply (le_antisymm _ _ H F);
+                           clear H; clear F
+    end
+  .
+
+  Ltac _gen_rel :=
+    match goal with
+    | [ H: _ = max ?n ?m |- _ ] =>
+        let nH := fresh in destruct (max_dec_bis n m) as [[nH ?]|[nH ?]];
+                           rewrite nH in *; clear nH; try _gen_rel
+    | [ |- _ = max ?n ?m ] =>
+        let nH := fresh in destruct (max_dec_bis n m) as [[nH ?]|[nH ?]];
+                           rewrite nH in *; clear nH; try _gen_rel
+    | [ H: ?e1 ==> ?t -| _, F: ?e2 <== ?t -| _ |- _ ] =>
+        let nH := fresh in assert (nH: determine e2 <= determine e1) by
+          apply (synth_check_determine_order H F (le_refl _)); try antisym
+    | [ H: ?e <== ?t -| _, F: ?t <= determine ?e |- _ ] =>
+        let nH := fresh in assert (nH: determine e = t) by
+          apply (synth_and_order H F)
+    end
+  .
+
+  Ltac _ts_gen :=
+    match goal with
+    | [ H: _ ==> ?t -| ?f |- _ ] =>
+        destruct (synth_must_be_determine H); subst; clear H
+    | [ H: _ <== ?t -| ?f |-  _ ] =>
+        apply check_root in H
+    | [ H: forall _ _ _ _, _ -> _ -> _ -> _ ==> _ -| _,
+          He: nth_error _ _ = Some ?e,
+          Ht: nth_error _ _ = Some ?t,
+          Hf: nth_error _ _ = Some ?f
+          |- _ ] => specialize (H _ _ _ _ He Ht Hf)
+    | [ H: nth_error _ _ = Some _ |- _ ] => rewrite H in *
+    end
+  .
+
+  Lemma spec_implies_ts: forall e f1,
+      propagate_def e f1 -> exists f2, agree e f1 f2 /\ exists t, e ==> t -| f2.
   Proof.
-    Ltac _gen_eq_spec_ts :=
-      match goal with
-      | [ F: _ @[_] = Some (EBinOp _ _), H: binop_propagate _ |- _ ] =>
-          destruct (H _ _ _ _ F)
-      | [ F: _ @[_] = Some (EUnOp _), H: unop_propagate _ |- _ ] =>
-          apply H in F
-      | [ F: _ @[_] = Some (ECast _), H: cast_propagate _ |- _ ] =>
-          apply H in F
-      | [ F: _ @[_] = Some (EComp _ _), H: comp_propagate _ |- _ ] =>
-          destruct (H _ _ _ _ F _ (eq_refl _))
-      | [ F: _ @[_] = Some (ELogic _ _), H: logic_propagate _ |- _ ] =>
-          destruct (H _ _ _ _ F)
-      | [ F: _ @[_] = Some (EReduction _), H: red_propagate _ |- _ ] =>
-          apply H in F
-      | [ F: _ @[_] = Some (EShift _ _), H: shift_propagate _ |- _ ] =>
-          destruct (H _ _ _ _ F)
-      | [ F: _ @[_] = Some (EAssign _ _), H: assign_propagate _ |- _ ] =>
-          specialize (H _ _ _ _ F _ (eq_refl _))
-      | [ F: _ @[_] = Some (EShiftAssign _ _), H: shiftassign_propagate _ |- _ ] =>
-          apply H in F
-      | [ F: _ @[_] = Some (ECond _ _ _), H: cond_propagate _ |- _ ] =>
-          destruct (H _ _ _ _ _ F) as [? [? ?]]
-      | [ G: nth_error _ _ = _, F: _ @[_] = Some (EConcat _),
-              H: concat_propagate _ |- _ ] =>
-          specialize (H _ _ _ F _ _ G)
-      | [ F: _ @[_] = Some (ERepl _ _), H: repl_propagate _ |- _ ] =>
-          specialize (H _ _ _ _ F)
-      end
-    .
-    Ltac _tac_spec_ts :=
-      match goal with
-      | [ H: ?x = ?n, G: _ <== ?n -| ?f |- ?f _ = Some ?x ] =>
-          rewrite H; apply (check_root G)
-      | [ H: ?x = ?n, G: _ ==> ?n -| ?f |- ?f _ = Some ?x ] =>
-          rewrite H; apply (synth_root G)
-      | [ H: ?x ==> _ -| ?f |- ?f [] = Some (determine ?x) ] =>
-          destruct (synth_must_be_determine H); assumption
-      end
-    .
-    induction p using path_ind; intros; propagate_def_split.
-    - rewrite (synth_root H0). unfold toplevel_propagate in HTopLevel.
-      rewrite HTopLevel in H2. subst. reflexivity.
-    - apply IsPath_chunk in H1. destruct H1 as [e' [He Hf]].
-      destruct (synth_sub_expr _ H0 He) as [t' [f' [[H3|H3] H4]]];
-        rewrite H4; specialize (IHp (sub_expr_valid _ _ He) (f1 e p) (eq_refl _));
+    intros. destruct (always_synth e) as [t [f Hs]]. exists f. split.
+    - subst. unfold agree. intros. prop_split. induction p using path_ind.
+      + repeat prop_gen_eq; try _gen_rel; repeat _ts_gen; congruence.
+      + apply IsPath_chunk in H0. destruct H0 as [e' [Hse Hp]].
+        destruct (synth_sub_expr _ Hs Hse) as [t' [f' [[H3|H3] H4]]];
+        rewrite H4; specialize (IHp (sub_expr_valid _ _ _ Hse));
         specialize (H4 []); rewrite app_nil_r in H4; simpl in H4; rewrite H4 in IHp;
-        destruct e'.
-      + inv Hf.
-      + _gen_eq_spec_ts; inv Hf; inv H3; inv IHp; simpl; _tac_spec_ts.
-      + _gen_eq_spec_ts; inv Hf; inv H3; inv IHp; simpl; _tac_spec_ts.
-      + _gen_eq_spec_ts. inv Hf; inv H3. simpl. rewrite He; simpl; _tac_spec_ts.
-      + _gen_eq_spec_ts; inv Hf; inv H3.
-        * rewrite (max_l _ _ (synth_check_determine_order H7 H10 (le_refl _))) in *.
-          rewrite H; simpl; _tac_spec_ts.
-        * rewrite (max_r _ _ (synth_check_determine_order H10 H7 (le_refl _))) in *.
-          rewrite H. destruct (synth_must_be_determine H10). simpl. rewrite <- H2.
-          apply (check_root H7).
-        * rewrite (max_l _ _ (synth_check_determine_order H7 H10 (le_refl _))) in *.
-          rewrite H1. destruct (synth_must_be_determine H7). simpl. rewrite <- H2.
-          apply (check_root H10).
-        * rewrite (max_r _ _ (synth_check_determine_order H10 H7 (le_refl _))) in *.
-          rewrite H1; simpl; _tac_spec_ts.
-      + _gen_eq_spec_ts; inv Hf; inv H3.
-        * rewrite H; simpl; _tac_spec_ts.
-        * rewrite H1; simpl; _tac_spec_ts.
-      + _gen_eq_spec_ts; inv Hf; inv H3. rewrite He; simpl; _tac_spec_ts.
-      + _gen_eq_spec_ts; inv Hf; inv H3; inv IHp; simpl; try _tac_spec_ts.
-        rewrite H1; simpl; _tac_spec_ts.
-      + _gen_eq_spec_ts; inv Hf; inv H3; simpl; rewrite HAssign.
-        * destruct (synth_determine e'). rewrite (max_r _ _ (synth_check_order H H7)).
-          apply (check_root H7).
-        * destruct (synth_must_be_determine H5). subst.
-          rewrite (max_l _ _ (lt_le_incl _ _ H8)). assumption.
-      + _gen_eq_spec_ts; inv Hf; inv H3; inv IHp; simpl. rewrite He; simpl; _tac_spec_ts.
-      + _gen_eq_spec_ts; inv Hf; inv H3; inv IHp; simpl; try _tac_spec_ts.
-        * rewrite H5; simpl; _tac_spec_ts.
-        * rewrite H5; simpl; _tac_spec_ts.
-      + inv Hf. _gen_eq_spec_ts. inv H3. repeat gen_nth. rewrite HConcat. simpl.
-        rewrite H. specialize (H5 _ _ _ _ H6 H2 H); simpl; _tac_spec_ts.
-      + _gen_eq_spec_ts; inv Hf; inv H3. simpl. rewrite HRepl; simpl; _tac_spec_ts.
-      + inv Hf.
-      + _gen_eq_spec_ts; inv Hf; inv H3; try (inv H2); inv IHp; simpl; _tac_spec_ts.
-      + _gen_eq_spec_ts; inv Hf; inv H3; try (inv H); inv IHp; simpl; _tac_spec_ts.
-      + _gen_eq_spec_ts; inv Hf; inv H3; inv H1; simpl; rewrite He; simpl; _tac_spec_ts.
-      + destruct (HComp _ _ _ _ He _ (eq_refl _)); inv Hf; inv H3; inv H5.
-        * rewrite (max_l _ _ (synth_check_determine_order H9 H12 (le_refl _))) in *.
-          rewrite H; simpl; _tac_spec_ts.
-        * rewrite (max_r _ _ (synth_check_determine_order H12 H9 (le_refl _))) in *.
-          rewrite H. destruct (synth_must_be_determine H12). simpl. rewrite <- H3.
-          apply (check_root H9).
-        * rewrite (max_l _ _ (synth_check_determine_order H9 H12 (le_refl _))) in *.
-          rewrite H1. destruct (synth_must_be_determine H9). simpl. rewrite <- H3.
-          apply (check_root H12).
-        * rewrite (max_r _ _ (synth_check_determine_order H12 H9 (le_refl _))) in *.
-          rewrite H1; simpl; _tac_spec_ts.
-      + _gen_eq_spec_ts; inv Hf; inv H3; inv H5.
-        * rewrite H; simpl; _tac_spec_ts.
-        * rewrite H1; simpl; _tac_spec_ts.
-      + _gen_eq_spec_ts; inv Hf; inv H3; inv H1; rewrite He; simpl; _tac_spec_ts.
-      + _gen_eq_spec_ts; inv Hf; inv H3; try (inv H2); inv IHp; simpl; try _tac_spec_ts.
-        rewrite H1. simpl; _tac_spec_ts.
-      + _gen_eq_spec_ts; inv Hf; inv H3; inv H2; simpl; rewrite HAssign.
-        * destruct (synth_determine e'). rewrite (max_r _ _ (synth_check_order H2 H9)).
-          apply (check_root H9).
-        * destruct (synth_must_be_determine H7). subst.
-          rewrite (max_l _ _ (lt_le_incl _ _ H10)). assumption.
-      + _gen_eq_spec_ts; inv Hf; inv H3; inv H2; inv IHp; simpl;
-        rewrite He; _tac_spec_ts.
-      + _gen_eq_spec_ts; inv Hf; inv H3; try (inv H2); inv IHp; simpl; try _tac_spec_ts.
-        rewrite H5; _tac_spec_ts.
-      + inv Hf. _gen_eq_spec_ts. inv H3. inv H1; repeat gen_nth. rewrite HConcat. simpl.
-        rewrite H1. specialize (H9 _ _ _ _ H6 H3 H1); _tac_spec_ts.
-      + _gen_eq_spec_ts; inv Hf; inv H3; inv H2; simpl. rewrite HRepl; _tac_spec_ts.
+          destruct e'; inv Hp; inv_ts; simpl in *; repeat prop_gen_eq; try _gen_rel;
+          repeat gen_nth; repeat _ts_gen; congruence || lia.
+    - exists t. assumption.
   Qed.
 
-  Theorem ts_implies_spec : forall f1,
-      propagate_def f1 -> forall e f2, e ==> (determine e) -| f2 ->
-                                 forall p, IsPath e p -> forall n, f2 p = Some n -> f1 e p = n.
+  Lemma ts_implies_spec: forall e f1 f2 t,
+      agree e f1 f2 -> e ==> t -| f2 -> propagate_def e f1.
   Proof.
-    induction p using path_ind; intros; propagate_def_split.
-    - destruct (synth_must_be_determine H0). rewrite H3 in H2. inv H2. apply HTopLevel.
-    - apply IsPath_chunk in H1. destruct H1 as [e' [He Hf]].
-      specialize (IHp (sub_expr_valid _ _ He)).
-      destruct (synth_sub_expr _ H0 He) as [t' [f' [[H3|H3] H4]]];
-        assert (Hf': f2 p = f' []) by
-        (specialize (H4 []); rewrite app_nil_r in H4; assumption);
-        rewrite H4 in H2; destruct e'.
-      + inv Hf.
-      + _gen_eq_spec_ts; inv Hf; inv H3; simpl in *; apply IHp in Hf'.
-        * apply synth_root in H8. congruence.
-        * apply check_root in H8. congruence.
-        * apply check_root in H11. congruence.
-        * apply synth_root in H11. congruence.
-      + _gen_eq_spec_ts. inv Hf. rewrite He. apply IHp. inv H3. simpl in *.
-        apply synth_root in H1. congruence.
-      + _gen_eq_spec_ts. inv Hf. rewrite He. inv H3. simpl in *.
-        destruct (synth_must_be_determine H1). congruence.
-      + _gen_eq_spec_ts. inv Hf; inv H3.
-        * rewrite (max_l _ _ (synth_check_determine_order H8 H11 (le_refl _))) in *.
-          destruct (synth_must_be_determine H8). simpl in *. congruence.
-        * rewrite (max_r _ _ (synth_check_determine_order H11 H8 (le_refl _))) in *.
-          destruct (synth_must_be_determine H11). simpl in *.
-          apply check_root in H8. congruence.
-        * rewrite (max_l _ _ (synth_check_determine_order H8 H11 (le_refl _))) in *.
-          destruct (synth_must_be_determine H8). simpl in *.
-          apply check_root in H11. congruence.
-        * rewrite (max_r _ _ (synth_check_determine_order H11 H8 (le_refl _))) in *.
-          destruct (synth_must_be_determine H11). simpl in *. congruence.
-      + _gen_eq_spec_ts; inv Hf; inv H3; simpl in *.
-        * destruct (synth_must_be_determine H8). congruence.
-        * destruct (synth_must_be_determine H11). congruence.
-      + _gen_eq_spec_ts; inv Hf; inv H3; simpl in *;
-        edestruct synth_must_be_determine; [ eassumption | congruence].
-      + _gen_eq_spec_ts; inv Hf; inv H3; simpl in *.
-        * apply synth_root in H8. specialize (IHp _ Hf'). congruence.
-        * edestruct synth_must_be_determine; [ eassumption | congruence].
-      + _gen_eq_spec_ts; inv Hf; inv H3; simpl in *; rewrite HAssign.
-        * destruct (synth_determine e'). rewrite (max_r _ _ (synth_check_order H H8)).
-          apply check_root in H8. congruence.
-        * destruct (synth_must_be_determine H6). subst.
-          rewrite (max_l _ _ (lt_le_incl _ _ H9)). congruence.
-      + _gen_eq_spec_ts; inv Hf; inv H3; simpl in *;
-        destruct (synth_must_be_determine H8); congruence.
-      + _gen_eq_spec_ts; inv Hf; inv H3; simpl in *; apply IHp in Hf'.
-        * destruct (synth_must_be_determine H10). congruence.
-        * destruct (synth_must_be_determine H10). congruence.
-        * apply synth_root in H13. congruence.
-        * apply check_root in H13. congruence.
-        * apply check_root in H14. congruence.
-        * apply synth_root in H14. congruence.
-      + inv Hf; _gen_eq_spec_ts; inv H3; inv H1; repeat gen_nth; simpl in *.
-        rewrite H1 in *. specialize (H8 _ _ _ _ H6 H H1).
-        destruct (synth_must_be_determine H8). congruence.
-      + _gen_eq_spec_ts; inv Hf; inv H3; simpl in *;
-        edestruct synth_must_be_determine; [ eassumption | congruence].
-      + inv Hf.
-      + _gen_eq_spec_ts; inv Hf; inv H3; try (inv H5); simpl in Hf'; apply IHp in Hf';
-        simpl in H2; subst.
-        * apply check_root in H8. congruence.
-        * apply check_root in H11. congruence.
-      + _gen_eq_spec_ts. inv Hf. rewrite He. apply IHp. inv H3. inv H.
-        simpl in *. apply check_root in H1. congruence.
-      + _gen_eq_spec_ts. inv Hf. rewrite He. inv H3. inv H1. simpl in *.
-        destruct (synth_must_be_determine H7). simpl in *. congruence.
-      + _gen_eq_spec_ts. inv Hf; inv H3; inv H7.
-        * rewrite (max_l _ _ (synth_check_determine_order H10 H13 (le_refl _))) in *.
-          destruct (synth_must_be_determine H10). simpl in *. congruence.
-        * rewrite (max_r _ _ (synth_check_determine_order H13 H10 (le_refl _))) in *.
-          destruct (synth_must_be_determine H13). simpl in *.
-          apply check_root in H10. congruence.
-        * rewrite (max_l _ _ (synth_check_determine_order H10 H13 (le_refl _))) in *.
-          destruct (synth_must_be_determine H10). simpl in *.
-          apply check_root in H13. congruence.
-        * rewrite (max_r _ _ (synth_check_determine_order H13 H10 (le_refl _))) in *.
-          destruct (synth_must_be_determine H13). simpl in *. congruence.
-      + _gen_eq_spec_ts; inv Hf; inv H3; inv H7; simpl in *.
-        * destruct (synth_must_be_determine H10). congruence.
-        * destruct (synth_must_be_determine H13). congruence.
-      + _gen_eq_spec_ts; inv Hf; inv H3; inv H1; simpl in *;
-        edestruct synth_must_be_determine; [ eassumption | congruence].
-      + _gen_eq_spec_ts; inv Hf; inv H3; try (inv H5); simpl in *.
-        * apply check_root in H8. specialize (IHp _ Hf'). congruence.
-        * edestruct synth_must_be_determine; [ eassumption | congruence].
-      + _gen_eq_spec_ts; inv Hf; inv H3; inv H5; simpl in *; rewrite HAssign.
-        * destruct (synth_determine e'). rewrite (max_r _ _ (synth_check_order H3 H10)).
-          apply check_root in H10. congruence.
-        * destruct (synth_must_be_determine H8). subst.
-          rewrite (max_l _ _ (lt_le_incl _ _ H11)). congruence.
-      + _gen_eq_spec_ts; inv Hf; inv H3; inv H5; simpl in *;
-        destruct (synth_must_be_determine H10); congruence.
-      + _gen_eq_spec_ts; inv Hf; inv H3; try (inv H6); simpl in *; apply IHp in Hf'.
-        * destruct (synth_must_be_determine H10). congruence.
-        * apply check_root in H13. congruence.
-        * apply check_root in H14. congruence.
-      + inv Hf; _gen_eq_spec_ts; inv H3; inv H1; repeat gen_nth; simpl in *.
-        rewrite H1 in *. specialize (H10 _ _ _ _ H6 H3 H1).
-        destruct (synth_must_be_determine H10). congruence.
-      + _gen_eq_spec_ts; inv Hf; inv H3; inv H5; simpl in *;
-        destruct (synth_must_be_determine H8); congruence.
+    Ltac _ts_spec :=
+      match goal with
+      | [ H: ?e @[?p] = Some _ |- ?f (?p ++ [?x]) = _ ] =>
+          assert (Hpx: IsPath e (p ++ [x])) by
+          (apply IsPath_chunk; eexists; split;
+           [apply H | econstructor; try eassumption; constructor]);
+          assert (Hp: IsPath e p) by apply (sub_expr_valid _ _ _ H)
+      | [ H: IsPath _ _, F: forall _, IsPath _ _ -> _ |- _ ] =>
+          apply F in H
+      | [ H: forall _,  _ = _ |- ?f (?p ++ [?x]) = _ ] =>
+          specialize (H []) as HNil; rewrite app_nil_r in *;
+          specialize (H [x]) as Hx
+      end
+    .
+    Ltac _crunch_ts_imp_spec :=
+      match goal with
+      | [ H: _ ==> _ -| _, F: _ @[_] = Some _ |- _ ] =>
+          destruct (synth_sub_expr _ H F) as [t' [f' [[H3|H3] H4]]];
+          repeat _ts_spec; inv_ts; simpl in *; repeat gen_nth; try _gen_rel;
+          repeat _ts_gen; congruence || lia
+      end
+    .
+    unfold agree. autounfold with Spec. repeat split; intros; try _crunch_ts_imp_spec.
+    destruct (synth_must_be_determine H0); specialize (H [] (P_Empty _)); congruence.
   Qed.
 
-  Theorem ts_equiv_spec : forall f1 f2 e,
-      propagate_def f1 -> e ==> (determine e) -| f2 ->
-      forall p, IsPath e p -> forall n, f2 p = Some n <-> f1 e p = n.
+  Theorem ts_equiv_spec : forall e f1,
+      propagate_def e f1 <-> exists f2, agree e f1 f2 /\ exists t, e ==> t -| f2.
   Proof.
     split; intros.
-    - apply (ts_implies_spec H H0 H1 H2).
-    - apply (spec_implies_ts H H0 H1 H2).
+    - apply (spec_implies_ts _ _ H).
+    - destruct H as [f2 [H1 [t H2]]]. apply (ts_implies_spec _ _ _ _ H1 H2).
   Qed.
 
 End Equiv.
-
