Rocq/src/Algo.v
@@ -1,0 +1,199 @@
+From Stdlib Require Import Lists.List.
+
+From Verilog Require Import Expr.
+From Verilog Require Import ExprPath.
+From Verilog Require Import TypedExpr.
+From Verilog Require Import TypedExprPath.
+From Verilog Require Import TypeSystem.
+From Verilog Require Import Spec.
+From Verilog Require Import Utils.
+
+Import ListNotations.
+
+
+Import Path.
+Import Expr.
+Import ExprPath.
+Import TypedExpr.
+Import TypedExprPath.
+Import TypeSystem.
+Import Spec.
+Import Utils.
+
+Module Algo.
+  Fixpoint down s e :=
+    match e with
+    | TAtom _ op => TAtom s op
+    | TBinOp _ tLhs tRhs => TBinOp s (down s tLhs) (down s tRhs)
+    | TUnOp _ tArg => TUnOp s (down s tArg)
+    | TCast _ tArg => TCast s tArg
+    | TComp _ tLhs tRhs => TComp s tLhs tRhs
+    | TLogic _ tLhs tRhs => TLogic s tLhs tRhs
+    | TReduction _ tArg => TReduction s tArg
+    | TShift _ tLhs tRhs => TShift s (down s tLhs) tRhs
+    | TAssign _ lval tArg => TAssign s lval tArg
+    | TShiftAssign _ lval tArg => TShiftAssign s lval tArg
+    | TCond _ tArg tLhs tRhs => TCond s tArg (down s tLhs) (down s tRhs)
+    | TConcat _ tArgs => TConcat s tArgs
+    | TRepl _ n tArg => TRepl s n tArg
+    end
+  .
+
+  Definition down_curry (x: nat * TypedExpr) := let (s, e) := x in down s e.
+
+  Fixpoint up e :=
+    match e with
+    | EAtom op => (op, TAtom op op)
+    | EBinOp lhs rhs =>
+        let (lhsS, uLhs) := up lhs in
+        let (rhsS, uRhs) := up rhs in
+        let s := max lhsS rhsS in
+        (s, TBinOp s uLhs uRhs)
+    | EUnOp arg =>
+        let (argS, uArg) := up arg in
+        (argS, TUnOp argS uArg)
+    | ECast arg =>
+        let (argS, uArg) := up arg in
+        let dArg := down argS uArg in
+        (argS, TUnOp argS dArg)
+    | EComp lhs rhs =>
+        let (lhsS, uLhs) := up lhs in
+        let (rhsS, uRhs) := up rhs in
+        let s := max lhsS rhsS in
+        let dLhs := down s uLhs in
+        let dRhs := down s uRhs in
+        (1, TComp 1 dLhs dRhs)
+    | ELogic lhs rhs =>
+        let (lhsS, uLhs) := up lhs in
+        let (rhsS, uRhs) := up rhs in
+        let dLhs := down lhsS uLhs in
+        let dRhs := down rhsS uRhs in
+        (1, TLogic 1 dLhs dRhs)
+    | EReduction arg =>
+        let (argS, uArg) := up arg in
+        let dArg := down argS uArg in
+        (1, TReduction 1 dArg)
+    | EShift lhs rhs =>
+        let (lhsS, uLhs) := up lhs in
+        let (rhsS, uRhs) := up rhs in
+        let dRhs := down rhsS uRhs in
+        (lhsS, TLogic lhsS uLhs dRhs)
+    | EAssign lval arg =>
+        let (argS, uArg) := up arg in
+        let s := max lval argS in
+        let dArg := down s uArg in
+        (lval, TAssign lval lval dArg)
+    | EShiftAssign lval arg =>
+        let (argS, uArg) := up arg in
+        let dArg := down argS uArg in
+        (lval, TAssign lval lval dArg)
+    | ECond arg lhs rhs =>
+        let (argS, uArg) := up arg in
+        let (lhsS, uLhs) := up lhs in
+        let (rhsS, uRhs) := up rhs in
+        let s := max lhsS rhsS in
+        let dArg := down argS uArg in
+        (s, TCond s dArg uLhs uRhs)
+    | EConcat args =>
+        let uArgs := map up args in
+        let dArgs := map down_curry uArgs in
+        let s := sum (map fst uArgs) in
+        (s, TConcat s dArgs)
+    | ERepl n arg =>
+        let (argS, uArg) := up arg in
+        let dArg := down argS uArg in
+        let s := n * argS in
+        (s, TReduction s dArg)
+    end
+  .
+
+  Definition type e := down_curry (up e).
+
+  Definition size_at e p := option_map size (e @@[p]).
+
+  Theorem down_shape : forall e p s, IsTypedPath e p <-> IsTypedPath (down s e) p.
+  Proof.
+    split; intros.
+    - induction H; simpl in *; econstructor; eassumption.
+    - generalize dependent p. induction e; intros; simpl in *;
+        try (inv H; constructor; firstorder).
+      inv H0. constructor. econstructor; eassumption.
+  Qed.
+
+  Theorem up_shape : forall e p, IsPath e p <-> IsTypedPath (snd (up e)) p.
+  Proof.
+    split; intros.
+    Ltac _up_shape :=
+      match goal with
+      | [ |- IsTypedPath (snd (let (_, _) := up ?e in _)) _ ] => destruct (up e)
+      | [ H: IsTypedPath (snd (let (_, _) := up ?e in _)) _ |- _ ] => destruct (up e)
+      | [ H: IsTypedPath (down _ _) _ |- _ ] => rewrite <- down_shape in H
+      end
+    .
+    - induction H; simpl in *; repeat _up_shape; simpl in *; try constructor;
+        try (apply down_shape); try assumption.
+      econstructor.
+      + repeat (rewrite nth_error_map). rewrite H. simpl in *. reflexivity.
+      + destruct (up e). simpl in *. apply down_shape. assumption.
+    - generalize dependent p. induction e; intros; simpl in *; repeat _up_shape;
+        simpl in *; try (inv H); try constructor; repeat _up_shape; try firstorder.
+      inv H0.
+      + constructor.
+      + repeat (rewrite nth_error_map in H3). destruct (nth_error args n) eqn:HArg;
+        inv H3. econstructor.
+        * eassumption.
+        * eapply H. eassumption. destruct (up e0). simpl in *.
+          rewrite <- down_shape in H5. assumption.
+  Qed.
+
+  Theorem type_shape : forall e p, IsPath e p <-> IsTypedPath (type e) p.
+  Proof.
+    intros. unfold type. destruct (up e) eqn:Hup. simpl. rewrite <- down_shape.
+    assert (Ht: t = snd (up e)) by (rewrite Hup; reflexivity). subst. apply up_shape.
+  Qed.
+
+  Hint Unfold type : core.
+  Hint Unfold size_at : core.
+  Hint Unfold down_curry : core.
+
+  Theorem up_size : forall e, fst (up e) = determine e.
+  Proof.
+    Ltac _up_size :=
+      match goal with
+      | [ |- fst (let (_, _) := up ?e in _) = _ ] => destruct (up e)
+      | [ H: fst (up ?e) = _ |- _ ] => destruct (up e)
+      end
+    .
+    induction e using Expr_ind; autounfold; simpl;
+      repeat _up_size; simpl in *; try congruence.
+    induction args.
+    - reflexivity.
+    - simpl. rewrite (H 0 _ (eq_refl _)). rewrite IHargs.
+      + reflexivity.
+      + intros n. apply (H (S n)).
+  Qed.
+
+  Theorem down_size : forall e s, size (down s e) = s.
+  Proof.
+    intros [] ?; reflexivity.
+  Qed.
+
+  Theorem type_size : forall e, size (type e) = determine e.
+  Proof.
+    intros. autounfold. destruct (up e) eqn:Hup.
+    assert (fst (up e) = n) by (rewrite Hup; reflexivity).
+    rewrite down_size. rewrite <- H. apply up_size.
+  Qed.
+
+  Theorem ttoreike : forall e t f,
+      e ==> t -| f -> forall p, IsPath e p -> size_at (type e) p = f p.
+  Proof.
+    intros. induction p using path_ind.
+    - unfold size_at. rewrite sub_typed_expr_nil. simpl. rewrite type_size.
+      destruct (synth_must_be_determine H). congruence.
+    - unfold size_at. admit.
+  Admitted.
+
+End Algo.
+
+
