Rocq/src/ExprPath.v
@@ -1,0 +1,142 @@
+From Stdlib Require Import Lists.List.
+
+From Verilog Require Import Expr.
+From Verilog Require Export Path.
+From Verilog Require Import Utils.
+
+Import ListNotations.
+
+Import Expr.
+Import Path.
+Import Utils.
+
+Module ExprPath.
+  Inductive IsPath : Expr -> path -> Prop :=
+  | P_Empty : forall e,
+      IsPath e []
+  | P_LhsBinOp : forall lhs rhs p,
+      IsPath lhs p -> IsPath (EBinOp lhs rhs) (Left :: p)
+  | P_RhsBinOp : forall lhs rhs p,
+      IsPath rhs p -> IsPath (EBinOp lhs rhs) (Right :: p)
+  | P_UnOpArg : forall arg p,
+      IsPath arg p -> IsPath (EUnOp arg) (Arg :: p)
+  | P_CastArg : forall arg p,
+      IsPath arg p -> IsPath (ECast arg) (Arg :: p)
+  | P_LhsCompOp : forall lhs rhs p,
+      IsPath lhs p -> IsPath (EComp lhs rhs) (Left :: p)
+  | P_RhsCompOp : forall lhs rhs p,
+      IsPath rhs p -> IsPath (EComp lhs rhs) (Right :: p)
+  | P_LhsLogic : forall lhs rhs p,
+      IsPath lhs p -> IsPath (ELogic lhs rhs) (Left :: p)
+  | P_RhsLogic : forall lhs rhs p,
+      IsPath rhs p -> IsPath (ELogic lhs rhs) (Right :: p)
+  | P_RedArg : forall arg p,
+      IsPath arg p -> IsPath (EReduction arg) (Arg :: p)
+  | P_LhsShift : forall lhs rhs p,
+      IsPath lhs p -> IsPath (EShift lhs rhs) (Left :: p)
+  | P_RhsShift : forall lhs rhs p,
+      IsPath rhs p -> IsPath (EShift lhs rhs) (Right :: p)
+  | P_AssignArg : forall op arg p,
+      IsPath arg p -> IsPath (EAssign op arg) (Arg :: p)
+  | P_ShiftAssignArg : forall op arg p,
+      IsPath arg p -> IsPath (EShiftAssign op arg) (Arg :: p)
+  | P_CondCond : forall cond tb fb p,
+      IsPath cond p -> IsPath (ECond cond tb fb) (Arg :: p)
+  | P_CondTrue : forall cond tb fb p,
+      IsPath tb p -> IsPath (ECond cond tb fb) (Left :: p)
+  | P_CondFalse : forall cond tb fb p,
+      IsPath fb p -> IsPath (ECond cond tb fb) (Right :: p)
+  | P_ConcatArgs : forall n args e p,
+      nth_error args n = Some e -> IsPath e p -> IsPath (EConcat args) (Args n :: p)
+  | P_ReplArg : forall i arg p,
+      IsPath arg p -> IsPath (ERepl i arg) (Arg :: p)
+  .
+
+  Fixpoint sub_expr (e: Expr) (p: path) :=
+    match e, p with
+    | e, [] => Some e
+    | EBinOp lhs _, Left :: p => sub_expr lhs p
+    | EBinOp _ rhs, Right :: p => sub_expr rhs p
+    | EUnOp arg, Arg :: p => sub_expr arg p
+    | ECast arg, Arg :: p => sub_expr arg p
+    | EComp lhs _, Left :: p => sub_expr lhs p
+    | EComp _ rhs, Right :: p => sub_expr rhs p
+    | ELogic lhs _, Left :: p => sub_expr lhs p
+    | ELogic _ rhs, Right :: p => sub_expr rhs p
+    | EReduction arg, Arg :: p => sub_expr arg p
+    | EShift lhs _, Left :: p => sub_expr lhs p
+    | EShift _ rhs, Right :: p => sub_expr rhs p
+    | EAssign _ arg, Arg :: p => sub_expr arg p
+    | EShiftAssign _ arg, Arg :: p => sub_expr arg p
+    | ECond cond _ _, Arg :: p => sub_expr cond p
+    | ECond _ tb _, Left :: p => sub_expr tb p
+    | ECond _ _ fb, Right :: p => sub_expr fb p
+    | EConcat args, Args i :: p =>
+        match nth_error args i with
+        | Some e => sub_expr e p
+        | None => None
+        end
+    | ERepl _ arg, Arg :: p => sub_expr arg p
+    | _, _ :: _ => None
+    end
+  .
+
+  Notation "e @[ p ]" := (sub_expr e p) (at level 20).
+
+  Lemma IsPath_is_sub_expr: forall e p, IsPath e p -> exists e0, e @[p] = Some e0.
+  Proof.
+    intros. induction H; try (destruct IHIsPath as [x H1]; exists x; assumption).
+    - exists e; destruct e; reflexivity.
+    - destruct IHIsPath as [x H1]; exists x. simpl. rewrite H. assumption.
+  Qed.
+
+  Lemma sub_expr_valid: forall e p f, e @[p] = Some f -> IsPath e p.
+  Proof.
+    induction e using Expr_ind; intros;
+      try (destruct p as [|[]]; try (discriminate H); constructor; firstorder).
+      - destruct p as [|[]]; try (discriminate H); try (discriminate H0).
+        + constructor.
+        + simpl in H0. destruct (nth_error args i) eqn:H1; try (discriminate H0).
+          econstructor. eassumption. apply (H _ _ H1 _ _ H0).
+  Qed.
+
+  Lemma IsPath_sub_expr_iff: forall e p, IsPath e p <-> exists e0, e @[p] = Some e0.
+  Proof.
+    split.
+    - apply IsPath_is_sub_expr.
+    - intros [? H]. apply (sub_expr_valid _ _ _ H).
+  Qed.
+
+  Lemma sub_expr_nil: forall e, e @[[]] = Some e.
+  Proof.
+    intros. destruct e; reflexivity.
+  Qed.
+
+  Lemma sub_exp_chunk : forall p q e g,
+      (exists f, e @[p] = Some f /\ f @[q] = Some g) <-> e @[p ++ q] = Some g.
+  Proof.
+    induction p; split; intros.
+    - destruct H as [f [H1 H2]]. rewrite sub_expr_nil in H1. inv H1. assumption.
+    - exists e. split. apply sub_expr_nil. assumption.
+    - destruct H as [f [H1 H2]]. destruct e; simpl; try (discriminate H1);
+        destruct a; simpl in *; try (destruct (nth_error _ i));
+        (apply IHp; exists f; intuition) || discriminate H1.
+    - destruct a; simpl in H;
+        try (destruct e; discriminate H || (apply IHp in H; assumption));
+        destruct e; discriminate H || (destruct (nth_error _ i) eqn:H';
+        discriminate H || (apply IHp in H; simpl; rewrite H'; assumption)).
+  Qed.
+
+  Lemma IsPath_chunk : forall e p c,
+      IsPath e (p ++ c) <-> (exists f, e @[p] = Some f /\ IsPath f c).
+  Proof.
+    split; intros.
+    - destruct (IsPath_is_sub_expr _ _ H) as [g H1]. apply sub_exp_chunk in H1.
+      destruct H1 as [f [H2 H3]]. exists f. split. assumption. apply IsPath_sub_expr_iff.
+      exists g. assumption.
+    - destruct H as [f [H1 H2]]. apply IsPath_sub_expr_iff.
+      apply IsPath_sub_expr_iff in H2. destruct H2 as [g H2]. exists g.
+      apply sub_exp_chunk. exists f. intuition.
+  Qed.
+
+End ExprPath.
