Rocq/src/Spec.v
@@ -1,17 +1,16 @@
 From Stdlib Require Import Lists.List.
 
 From Verilog Require Import Expr.
-From Verilog Require Import Path.
+From Verilog Require Import ExprPath.
 From Verilog Require Import Utils.
 
 Import ListNotations.
 Import Nat.
 
 Import Expr.
+Import ExprPath.
 Import Path.
 Import Utils.
-
-Set Implicit Arguments.
 
 Module Spec.
 
@@ -34,66 +33,67 @@ Module Spec.
       end
     .
 
-    Variable propagate : Expr -> path -> nat.
+    Variable e : Expr.
+    Variable propagate : path -> nat.
 
-    Definition binop_propagate := forall e p lhs rhs,
+    Definition binop_propagate := forall p lhs rhs,
         e @[p] = Some (EBinOp lhs rhs) ->
-        propagate e (p ++ [Left]) = propagate e p /\
-          propagate e (p ++ [Right]) = propagate e p.
+        propagate (p ++ [Left]) = propagate p /\
+          propagate (p ++ [Right]) = propagate p.
 
-    Definition unop_propagate := forall e p arg,
+    Definition unop_propagate := forall p arg,
         e @[p] = Some (EUnOp arg) ->
-        propagate e (p ++ [Arg]) = propagate e p.
+        propagate (p ++ [Arg]) = propagate p.
 
-    Definition cast_propagate := forall e p arg,
+    Definition cast_propagate := forall p arg,
         e @[p] = Some (ECast arg) ->
-        propagate e (p ++ [Arg]) = determine arg.
+        propagate (p ++ [Arg]) = determine arg.
 
-    Definition comp_propagate := forall e p lhs rhs,
+    Definition comp_propagate := forall p lhs rhs,
         e @[p] = Some (EComp lhs rhs) ->
         forall s, s = max (determine lhs) (determine rhs) ->
-             propagate e (p ++ [Left]) = s /\
-               propagate e (p ++ [Right]) = s.
+             propagate (p ++ [Left]) = s /\
+               propagate (p ++ [Right]) = s.
 
-    Definition logic_propagate := forall e p lhs rhs,
+    Definition logic_propagate := forall p lhs rhs,
         e @[p] = Some (ELogic lhs rhs) ->
-        propagate e (p ++ [Left]) = determine lhs /\
-          propagate e (p ++ [Right]) = determine rhs.
+        propagate (p ++ [Left]) = determine lhs /\
+          propagate (p ++ [Right]) = determine rhs.
 
-    Definition red_propagate := forall e p arg,
+    Definition red_propagate := forall p arg,
         e @[p] = Some (EReduction arg) ->
-        propagate e (p ++ [Arg]) = determine arg.
+        propagate (p ++ [Arg]) = determine arg.
 
-    Definition shift_propagate := forall e p lhs rhs,
+    Definition shift_propagate := forall p lhs rhs,
         e @[p] = Some (EShift lhs rhs) ->
-        propagate e (p ++ [Left]) = propagate e p /\
-          propagate e (p ++ [Right]) = determine rhs.
+        propagate (p ++ [Left]) = propagate p /\
+          propagate (p ++ [Right]) = determine rhs.
 
-    Definition assign_propagate := forall e p lval arg,
+    Definition assign_propagate := forall p lval arg,
         e @[p] = Some (EAssign lval arg) ->
         forall s, s = max (determine arg) lval ->
-             propagate e (p ++ [Arg]) = s.
+             propagate (p ++ [Arg]) = s.
 
-    Definition shiftassign_propagate := forall e p lval arg,
+    Definition shiftassign_propagate := forall p lval arg,
         e @[p] = Some (EShiftAssign lval arg) ->
-        propagate e (p ++ [Arg]) = determine arg.
+        propagate (p ++ [Arg]) = determine arg.
 
-    Definition cond_propagate := forall e p cond lhs rhs,
+    Definition cond_propagate := forall p cond lhs rhs,
         e @[p] = Some (ECond cond lhs rhs) ->
-        propagate e (p ++ [Left]) = propagate e p /\
-          propagate e (p ++ [Right]) = propagate e p /\
-          propagate e (p ++ [Arg]) = determine cond.
+        propagate (p ++ [Left]) = propagate p /\
+          propagate (p ++ [Right]) = propagate p /\
+          propagate (p ++ [Arg]) = determine cond.
 
-    Definition concat_propagate := forall e p args,
+    Definition concat_propagate := forall p args,
         e @[p] = Some (EConcat args) ->
         forall i f, nth_error args i = Some f ->
-               propagate e (p ++ [Args i]) = determine f.
+               propagate (p ++ [Args i]) = determine f.
 
-    Definition repl_propagate := forall e p i arg,
+    Definition repl_propagate := forall p i arg,
         e @[p] = Some (ERepl i arg) ->
-        propagate e (p ++ [Arg]) = determine arg.
+        propagate (p ++ [Arg]) = determine arg.
 
-    Definition toplevel_propagate := forall e, propagate e [] = determine e.
+    Definition toplevel_propagate := propagate [] = determine e.
 
     Definition propagate_def :=
       toplevel_propagate /\ binop_propagate /\ unop_propagate /\ cast_propagate /\
@@ -102,79 +102,82 @@ Module Spec.
         concat_propagate /\ repl_propagate.
   End SpecDef.
 
-  Theorem propagate_val : forall f, propagate_def f -> forall p e, IsPath e p -> exists n, f e p = n.
-  Proof.
-    induction p using path_ind; intros.
-    - firstorder.
-    - assert (He: IsPath e p /\ exists f, e @[p] = Some f /\ IsPath f [x]).
-      + split. apply (IsPath_prefix _ _ H0). apply IsPath_chunk. assumption.
-      + destruct He as [H1 [expr [H2 H3]]].
-        destruct expr; inv H3; destruct (IHp _ H1); try (eexists; firstorder).
-  Qed.
+  Create HintDb Spec discriminated.
 
-  Ltac propagate_def_split :=
+  Hint Unfold toplevel_propagate : Spec.
+  Hint Unfold binop_propagate : Spec.
+  Hint Unfold unop_propagate : Spec.
+  Hint Unfold cast_propagate : Spec.
+  Hint Unfold comp_propagate : Spec.
+  Hint Unfold logic_propagate : Spec.
+  Hint Unfold red_propagate : Spec.
+  Hint Unfold shift_propagate : Spec.
+  Hint Unfold assign_propagate : Spec.
+  Hint Unfold shiftassign_propagate : Spec.
+  Hint Unfold cond_propagate : Spec.
+  Hint Unfold concat_propagate : Spec.
+  Hint Unfold repl_propagate : Spec.
+
+  Hint Unfold propagate_def : Spec.
+
+
+  Ltac prop_split :=
     match goal with
-    | [ H: propagate_def _ |- _ ] =>
+    | [ H: propagate_def _ _ |- _ ] =>
         destruct H as [?HTopLevel [?HBinOp [?HUnOp [?HCast [?HComp [?HLogic [?HRed [?HShift [?HAssign [?HShiftAssign [?HCond [?HConcat ?HRepl]]]]]]]]]]]]
     end
   .
 
-  Theorem propagate_unique : forall p e,
-      IsPath e p -> forall f1 f2, propagate_def f1 -> propagate_def f2 -> f1 e p = f2 e p.
+  Ltac prop_gen_eq :=
+    match goal with
+    | [ H: toplevel_propagate _ _ |- _ ] =>
+        unfold toplevel_propagate in H
+    | [ F: _ @[_] = Some (EBinOp _ _), H: binop_propagate _ _ |- _ ] =>
+        specialize (H _ _ _ F); destruct H
+    | [ F: _ @[_] = Some (EUnOp _), H: unop_propagate _ _ |- _ ] =>
+        specialize (H _ _ F)
+    | [ F: _ @[_] = Some (ECast _), H: cast_propagate _ _ |- _ ] =>
+        specialize (H _ _ F)
+    | [ F: _ @[_] = Some (EComp _ _), H: comp_propagate _ _ |- _ ] =>
+        specialize (H _ _ _ F _ (eq_refl _)); destruct H
+    | [ F: _ @[_] = Some (ELogic _ _), H: logic_propagate _ _ |- _ ] =>
+        specialize (H _ _ _ F); destruct H
+    | [ F: _ @[_] = Some (EReduction _), H: red_propagate _ _ |- _ ] =>
+        specialize (H _ _ F)
+    | [ F: _ @[_] = Some (EShift _ _), H: shift_propagate _ _ |- _ ] =>
+        specialize (H _ _ _ F); destruct H
+    | [ F: _ @[_] = Some (EAssign _ _), H: assign_propagate _ _ |- _ ] =>
+        specialize (H _ _ _ F _ (eq_refl _))
+    | [ F: _ @[_] = Some (EShiftAssign _ _), H: shiftassign_propagate _ _ |- _ ] =>
+        specialize (H _ _ _ F)
+    | [ F: _ @[_] = Some (ECond _ _ _), H: cond_propagate _ _ |- _ ] =>
+        specialize (H _ _ _ _ F); destruct H as [? [? ?]]
+    | [ G: nth_error _ _ = _, F: _ @[_] = Some (EConcat _),
+            H: concat_propagate _ _ |- _ ] =>
+        specialize (H _ _ F _ _ G)
+    | [ F: _ @[_] = Some (ERepl _ _), H: repl_propagate _ _ |- _ ] =>
+        specialize (H _ _ _ F)
+    end
+  .
+
+  Theorem propagate_val : forall e f, propagate_def e f -> forall p, IsPath e p -> exists n, f p = n.
   Proof.
-    Ltac _propagate_unique_tac :=
-      match goal with
-      | [ G: _ _ _ = _ _ _, F: _ @[_] = Some (EBinOp _ _), H: binop_propagate _ |- _ ] =>
-          destruct (H _ _ _ _ F); rewrite G in *; assumption
-      | [ G: _ _ _ = _ _ _, F: _ @[_] = Some (EUnOp _), H: unop_propagate _ |- _ ] =>
-          apply H in F; rewrite G in *; assumption
-      | [ F: _ @[_] = Some (ELogic _ _), H: logic_propagate _ |- _ ] =>
-          destruct (H _ _ _ _ F); assumption
-      | [ F: _ @[_] = Some (EReduction _), H: red_propagate _ |- _ ] =>
-          apply H in F; assumption
-      | [ G: _ _ _ = _ _ _, F: _ @[_] = Some (EShift _ _), H: shift_propagate _ |- _ ] =>
-          destruct (H _ _ _ _ F); assumption || rewrite G in *; assumption
-      | [ F: _ @[_] = Some (EAssign _ _), H: assign_propagate _ |- _ ] =>
-          apply (H _ _ _ _ F); reflexivity
-      | [ F: _ @[_] = Some (EShiftAssign _ _), H: shiftassign_propagate _ |- _ ] =>
-          apply (H _ _ _ _ F)
-      | [ G: _ _ _ = _ _ _, F: _ @[_] = Some (ECond _ _ _), H: cond_propagate _ |- _ ] =>
-          destruct (H _ _ _ _ _ F) as [? []]; assumption || rewrite G in *; assumption
-      | [ G: nth_error _ _ = _, F: _ @[_] = Some (EConcat _),
-              H: concat_propagate _ |- _ ] => apply (H _ _ _ F _ _ G)
-      | [ F: _ @[_] = Some (ERepl _ _), H: repl_propagate _ |- _ ] =>
-          apply (H _ _ _ _ F)
-      end
-    .
-    assert (Heq: forall x y m : nat, x = m -> y = m -> x = y). { intros. subst. reflexivity. }
+    induction p using path_ind; intros.
+    - firstorder.
+    - rewrite IsPath_chunk in H0. destruct H0 as [expr [H2 H3]].
+      assert (He: IsPath e p) by apply (sub_expr_valid _ _ _ H2).
+      destruct expr; inv H3; destruct (IHp He); eexists; firstorder.
+  Qed.
+
+  Theorem propagate_unique :
+    forall e f1 f2, propagate_def e f1 -> propagate_def e f2 ->
+               forall p, IsPath e p -> f1 p = f2 p.
+  Proof.
     induction p using path_ind; intros.
     - apply eq_trans with (y := determine e). firstorder. symmetry. firstorder.
-    - assert (He: IsPath e p /\ exists f, e @[p] = Some f /\ IsPath f [x]).
-      + split. apply (IsPath_prefix _ _ H). apply IsPath_chunk. assumption.
-      + destruct He as [H2 [expr [H3 H4]]].
-        assert (Hf: f1 e p = f2 e p). apply (IHp _ H2 _ _ H0 H1). clear IHp.
-        destruct expr; inv H4; repeat propagate_def_split.
-        * apply Heq with (m := f1 e p); _propagate_unique_tac.
-        * apply Heq with (m := f1 e p); _propagate_unique_tac.
-        * apply Heq with (m := f1 e p); _propagate_unique_tac.
-        * apply Heq with (m := determine expr); firstorder.
-        * apply Heq with (m := max (determine expr1) (determine expr2)).
-          destruct (HComp0 _ _ _ _ H3 (max (determine expr1) (determine expr2))); auto.
-          destruct (HComp _ _ _ _ H3 (max (determine expr1) (determine expr2))); auto.
-        * apply eq_trans with (y := max (determine expr1) (determine expr2)).
-          destruct (HComp0 _ _ _ _ H3 (max (determine expr1) (determine expr2))); auto.
-          destruct (HComp _ _ _ _ H3 (max (determine expr1) (determine expr2))); auto.
-        * apply Heq with (m := determine expr1); _propagate_unique_tac.
-        * apply Heq with (m := determine expr2); _propagate_unique_tac.
-        * apply Heq with (m := determine expr); _propagate_unique_tac.
-        * apply Heq with (m := f1 e p); _propagate_unique_tac.
-        * apply Heq with (m := determine expr2); _propagate_unique_tac.
-        * apply Heq with (m := max (determine expr) lval); _propagate_unique_tac.
-        * apply Heq with (m := determine expr); _propagate_unique_tac.
-        * apply Heq with (m := determine expr1); _propagate_unique_tac.
-        * apply Heq with (m := f1 e p); _propagate_unique_tac.
-        * apply Heq with (m := f1 e p); _propagate_unique_tac.
-        * apply Heq with (m := determine e0); _propagate_unique_tac.
-        * apply Heq with (m := determine expr); _propagate_unique_tac.
+    - rewrite IsPath_chunk in H1. destruct H1 as [expr [H3 H4]].
+      specialize (IHp (sub_expr_valid _ _ _ H3)).
+      destruct expr; inv H4; repeat prop_split; repeat prop_gen_eq; congruence.
   Qed.
 End Spec.
+
