Rocq/src/TypedExprPath.v
@@ -1,0 +1,144 @@
+From Stdlib Require Import Lists.List.
+
+From Verilog Require Import TypedExpr.
+From Verilog Require Export Path.
+From Verilog Require Import Utils.
+
+Import ListNotations.
+
+Import TypedExpr.
+Import Path.
+Import Utils.
+
+Module TypedExprPath.
+  Inductive IsTypedPath : TypedExpr -> path -> Prop :=
+  | TP_Empty : forall e,
+      IsTypedPath e []
+  | TP_LhsBinOp : forall s lhs rhs p,
+      IsTypedPath lhs p -> IsTypedPath (TBinOp s lhs rhs) (Left :: p)
+  | TP_RhsBinOp : forall s lhs rhs p,
+      IsTypedPath rhs p -> IsTypedPath (TBinOp s lhs rhs) (Right :: p)
+  | TP_UnOpArg : forall s arg p,
+      IsTypedPath arg p -> IsTypedPath (TUnOp s arg) (Arg :: p)
+  | TP_CastArg : forall s arg p,
+      IsTypedPath arg p -> IsTypedPath (TCast s arg) (Arg :: p)
+  | TP_LhsCompOp : forall s lhs rhs p,
+      IsTypedPath lhs p -> IsTypedPath (TComp s lhs rhs) (Left :: p)
+  | TP_RhsCompOp : forall s lhs rhs p,
+      IsTypedPath rhs p -> IsTypedPath (TComp s lhs rhs) (Right :: p)
+  | TP_LhsLogic : forall s lhs rhs p,
+      IsTypedPath lhs p -> IsTypedPath (TLogic s lhs rhs) (Left :: p)
+  | TP_RhsLogic : forall s lhs rhs p,
+      IsTypedPath rhs p -> IsTypedPath (TLogic s lhs rhs) (Right :: p)
+  | TP_RedArg : forall s arg p,
+      IsTypedPath arg p -> IsTypedPath (TReduction s arg) (Arg :: p)
+  | TP_LhsShift : forall s lhs rhs p,
+      IsTypedPath lhs p -> IsTypedPath (TShift s lhs rhs) (Left :: p)
+  | TP_RhsShift : forall s lhs rhs p,
+      IsTypedPath rhs p -> IsTypedPath (TShift s lhs rhs) (Right :: p)
+  | TP_AssignArg : forall s op arg p,
+      IsTypedPath arg p -> IsTypedPath (TAssign s op arg) (Arg :: p)
+  | TP_ShiftAssignArg : forall s op arg p,
+      IsTypedPath arg p -> IsTypedPath (TShiftAssign s op arg) (Arg :: p)
+  | TP_CondCond : forall s cond tb fb p,
+      IsTypedPath cond p -> IsTypedPath (TCond s cond tb fb) (Arg :: p)
+  | TP_CondTrue : forall s cond tb fb p,
+      IsTypedPath tb p -> IsTypedPath (TCond s cond tb fb) (Left :: p)
+  | TP_CondFalse : forall s cond tb fb p,
+      IsTypedPath fb p -> IsTypedPath (TCond s cond tb fb) (Right :: p)
+  | TP_ConcatArgs : forall s n args e p,
+      nth_error args n = Some e -> IsTypedPath e p ->
+      IsTypedPath (TConcat s args) (Args n :: p)
+  | TP_ReplArg : forall s i arg p,
+      IsTypedPath arg p -> IsTypedPath (TRepl s i arg) (Arg :: p)
+  .
+
+  Fixpoint sub_typed_expr (e: TypedExpr) (p: path) :=
+    match e, p with
+    | e, [] => Some e
+    | TBinOp _ lhs _, Left :: p => sub_typed_expr lhs p
+    | TBinOp _ _ rhs, Right :: p => sub_typed_expr rhs p
+    | TUnOp _ arg, Arg :: p => sub_typed_expr arg p
+    | TCast _ arg, Arg :: p => sub_typed_expr arg p
+    | TComp _ lhs _, Left :: p => sub_typed_expr lhs p
+    | TComp _ _ rhs, Right :: p => sub_typed_expr rhs p
+    | TLogic _ lhs _, Left :: p => sub_typed_expr lhs p
+    | TLogic _ _ rhs, Right :: p => sub_typed_expr rhs p
+    | TReduction _ arg, Arg :: p => sub_typed_expr arg p
+    | TShift _ lhs _, Left :: p => sub_typed_expr lhs p
+    | TShift _ _ rhs, Right :: p => sub_typed_expr rhs p
+    | TAssign _ _ arg, Arg :: p => sub_typed_expr arg p
+    | TShiftAssign _ _ arg, Arg :: p => sub_typed_expr arg p
+    | TCond _ cond _ _, Arg :: p => sub_typed_expr cond p
+    | TCond _ _ tb _, Left :: p => sub_typed_expr tb p
+    | TCond _ _ _ fb, Right :: p => sub_typed_expr fb p
+    | TConcat _ args, Args i :: p =>
+        match nth_error args i with
+        | Some e => sub_typed_expr e p
+        | None => None
+        end
+    | TRepl _ _ arg, Arg :: p => sub_typed_expr arg p
+    | _, _ :: _ => None
+    end
+  .
+
+  Notation "e @@[ p ]" := (sub_typed_expr e p) (at level 20).
+
+  Lemma IsTypedPath_is_sub_typed_expr: forall e p, IsTypedPath e p -> exists e0, e @@[p] = Some e0.
+  Proof.
+    intros. induction H; try (destruct IHIsTypedPath as [x H1]; exists x; assumption).
+    - exists e; destruct e; reflexivity.
+    - destruct IHIsTypedPath as [x H1]; exists x. simpl. rewrite H. assumption.
+  Qed.
+
+  Lemma sub_typed_expr_valid: forall e p f, e @@[p] = Some f -> IsTypedPath e p.
+  Proof.
+    induction e using TypedExpr_ind; intros;
+      try (destruct p as [|[]]; try (discriminate H); constructor; firstorder).
+      - destruct p as [|[]]; try (discriminate H); try (discriminate H0).
+        + constructor.
+        + simpl in H0. destruct (nth_error args i) eqn:H1; try (discriminate H0).
+          econstructor. eassumption. apply (H _ _ H1 _ _ H0).
+  Qed.
+
+  Lemma IsTypedPath_sub_typed_expr_iff: forall e p, IsTypedPath e p <-> exists e0, e @@[p] = Some e0.
+  Proof.
+    split.
+    - apply IsTypedPath_is_sub_typed_expr.
+    - intros [? H]. apply (sub_typed_expr_valid _ _ _ H).
+  Qed.
+
+  Lemma sub_typed_expr_nil: forall e, e @@[ [] ] = Some e.
+  Proof.
+    intros. destruct e; reflexivity.
+  Qed.
+
+  Lemma sub_exp_chunk : forall p q e g,
+      (exists f, e @@[p] = Some f /\ f @@[q] = Some g) <-> e @@[p ++ q] = Some g.
+  Proof.
+    induction p; split; intros.
+    - destruct H as [f [H1 H2]]. rewrite sub_typed_expr_nil in H1. inv H1. assumption.
+    - exists e. split. apply sub_typed_expr_nil. assumption.
+    - destruct H as [f [H1 H2]]. destruct e; simpl; try (discriminate H1);
+        destruct a; simpl in *; try (destruct (nth_error _ i));
+        (apply IHp; exists f; intuition) || discriminate H1.
+    - destruct a; simpl in H;
+        try (destruct e; discriminate H || (apply IHp in H; assumption));
+        destruct e; discriminate H || (destruct (nth_error _ i) eqn:H';
+        discriminate H || (apply IHp in H; simpl; rewrite H'; assumption)).
+  Qed.
+
+  Lemma IsTypedPath_chunk : forall e p c,
+      IsTypedPath e (p ++ c) <-> (exists f, e @@[p] = Some f /\ IsTypedPath f c).
+  Proof.
+    split; intros.
+    - destruct (IsTypedPath_is_sub_typed_expr _ _ H) as [g H1].
+      apply sub_exp_chunk in H1. destruct H1 as [f [H2 H3]].
+      exists f. split. assumption. apply IsTypedPath_sub_typed_expr_iff.
+      exists g. assumption.
+    - destruct H as [f [H1 H2]]. apply IsTypedPath_sub_typed_expr_iff.
+      apply IsTypedPath_sub_typed_expr_iff in H2. destruct H2 as [g H2]. exists g.
+      apply sub_exp_chunk. exists f. intuition.
+  Qed.
+
+End TypedExprPath.
