Rocq/scripts/generate_doc.sh
@@ -1,3 +1,0 @@
-#!/bin/bash
-mkdir -p doc
-coqdoc --html -d doc -R _build/default/src Verilog _build/default/src/*.v
